inline-method works again

ElGamal.thy
@@ -73,10 +73,10 @@ procedure CPA_main :: "('pk,'sk,'m,'c) EncScheme * ('pk,'sk,'m,'c) CPA_Adv =proc
 subsection {* ElGamal *}
 
 definition (in group) ElGamal :: "('G,nat,'G,'G\<times>'G) EncScheme" where
- "ElGamal = LOCAL pk m0 c1 c2 sk sk' y gm gy.
+ "ElGamal = LOCAL pk m0 c1x c2x sk sk' y gm gy.
    Abs_EncScheme (proc() { sk <- uniform {0..<q}; return (g^sk, sk) },
                   proc(pk,m0) { y <- uniform {0..<q}; return (g^y, pk^y * m0) },
-                  proc(sk',(c1,c2)) { gy := c1; gm := c2; return Some (gm * inverse (gy^sk')) })"
+                  proc(sk',(c1x,c2x)) { gy := c1x; gm := c2x; return Some (gm * inverse (gy^sk')) })"
 
 
 procedure Correctness :: "(_,_,_,_) EncScheme =proc=> (_,bool)procedure" where
@@ -111,56 +111,19 @@ ML {*
 Procs_Typed.get_procedure_info @{context} true @{term "Correctness<$>ElGamal"}
 *}
 
-find_theorems "(p_vars (variable_pattern (_)))"
 
-(* TODO move *)
-lemma mk_expression_untyped_const_expression:
-  "mk_expression_untyped (const_expression (x::'a)) = const_expression_untyped (Type TYPE('a)) (embedding x)"
-  unfolding const_expression_def const_expression_untyped_def mk_expression_untyped_def e_fun_def e_vars_def
-  by (subst Abs_expression_inverse, auto?)+
 
-definition "assign_default_typed_rev vs = assign_default_typed (rev vs)"
-lemma assign_default_typed_rev: "assign_default_typed vs = assign_default_typed_rev (rev vs)"
-unfolding assign_default_typed_rev_def by auto
-
-lemma "assign_default_typed ([mk_variable_untyped a,mk_variable_untyped b,mk_variable_untyped c]) =
-  PROGRAM [ skip; a:=default; b:=default; c:=default ]"
-  unfolding assign_default_typed_def assign_default_def program_def seq_def assign_def
-      variable_pattern_def mk_expression_untyped_const_expression 
-  apply (subst Abs_program_inverse, tactic \<open>Skip_Proof.cheat_tac @{context} 1\<close>)+
-  apply (subst Abs_pattern_inverse, tactic \<open>Skip_Proof.cheat_tac @{context} 1\<close>)+
-  by simp
-
-lemma assign_default_typed_rev_cons: "assign_default_typed_rev (mk_variable_untyped v # vs) = seq (assign_default_typed_rev vs) (assign (variable_pattern v) (const_expression default))"
-  unfolding assign_default_typed_def assign_default_typed_rev_def assign_default_def seq_def
-    assign_def variable_pattern_def mk_expression_untyped_const_expression
-  apply simp
-  apply (subst Abs_program_inverse)
-   using assign_default_def assign_default_welltyped close auto
-  apply (subst Abs_program_inverse)
-   close (simp add: embedding_Type eu_type_const_expression_untyped)
-  apply (subst Abs_pattern_inverse)
-   by auto
-
-lemma assign_default_typed_rev_nil: "assign_default_typed_rev [] = Lang_Typed.skip"
-  unfolding assign_default_typed_def assign_default_typed_rev_def assign_default_def skip_def
-  by auto
 
 lemma correctness:
   shows "LOCAL succ0. hoare {True} succ0 := call Correctness <$> ElGamal(m) {succ0}"
 apply (inline "Correctness<$>ElGamal")
-(* TODO remove *) apply (simp add: assign_default_typed_rev assign_default_typed_rev_cons assign_default_typed_rev_nil)
 apply (inline "keygen<$>ElGamal")
-(* TODO remove *) apply (simp add: assign_default_typed_rev assign_default_typed_rev_cons assign_default_typed_rev_nil)
 apply (inline "dec<$>ElGamal")
 apply (inline "enc<$>ElGamal")
-apply (wp sample) apply skip apply autox
+apply (wp sample) apply skip apply auto
 unfolding power_mult[symmetric] apply (subst mult.commute[where 'a=nat]) 
 apply (subst mult.commute[where 'a='G]) apply (subst mult.assoc) by simp
 
 end (* context: group *)
-
-
-
-
+                                                   
 end (* theory *)
